%---------------------------------------------------------------------------
%	Packages
%---------------------------------------------------------------------------
\documentclass[10pt]{article}
\usepackage[utf8]{inputenc}
\usepackage[english]{babel}
\usepackage{multicol}
\usepackage{enumerate}
\usepackage{calc}
\usepackage{amsmath,amsthm,amsfonts,amssymb}
\usepackage{color,graphicx,overpic}
\usepackage{hyperref}
\usepackage[margin=0.70in]{geometry}
%---------------------------------------------------------------------------
%	Document
%---------------------------------------------------------------------------
\begin{document}
%---------------------------------------------------------------------------
%	General Equations
%---------------------------------------------------------------------------
\begin{center}
\underline{\textbf{General Equations}}
\end{center}
\begin{multicols}{3}
\begin{equation*}
\hat{H}\Psi=E\Psi
\end{equation*}
\begin{equation*}
i\hbar\frac{\partial \Psi}{\partial t}=\frac{-\hbar^2}{2m}\frac{\partial^2\Psi}{\partial x^2}+V\Psi
\end{equation*}
\begin{equation*}
i\hbar\frac{\partial \Psi}{\partial t}=\frac{-\hbar^2}{2m}\nabla^2\Psi+V\Psi
\end{equation*}
\begin{equation*}
\frac{-\hbar^2}{2m}\frac{\partial^2\Psi}{\partial x^2}+V\Psi=E\Psi
\end{equation*}
\begin{equation*}
\frac{-\hbar^2}{2m}\nabla^2\Psi+V\Psi=E\Psi
\end{equation*}
\begin{equation*}
\eta=\int_{-\infty}^{\infty} |\Psi(x,0)^{*}\Psi(x,0)|  \ dx=1
\end{equation*}
\begin{equation*}
\mathcal{O}=\int_{-\infty}^{\infty}\Psi(x,0)^*\Psi(x,0) \ dx
\end{equation*}
\begin{equation*}
P=\int_{a}^{b}\rho (x)  \ dx
\end{equation*}
\begin{equation*}
P_n=|C_n|^2
\end{equation*}
\begin{equation*}
<\hat{Q}>=\int \Psi^{*}\hat{Q}\Psi  \ dx=<\Psi|\hat{Q}\Psi>
\end{equation*}
\begin{equation*}
<x>=\int_{-\infty}^{\infty}x|\Psi(x,t)|^2 \ dx
\end{equation*}
\begin{equation*}
<x^2>=\int_{-\infty}^{\infty}x^2|\Psi(x,t)|^2 \ dx
\end{equation*}
\begin{equation*}
<\hat{p}>=m\frac{d<x>}{dt}=-i\hbar \int \left(\Psi^{*}\frac{\partial \Psi}{\partial x}\right)\Psi \ dx
\end{equation*}
\begin{equation*}
<\hat{p}^2>=\int \Psi^{*}\left(-\hbar^2\frac{\partial^2}{\partial x^2}\right)\Psi  \ dx
\end{equation*}
\begin{equation*}
<\hat{Q}(x,p)>=\int \Psi^{*}Q\left(x,\frac{\hbar}{i}\frac{\partial}{\partial x}\right)\Psi  \ dx
\end{equation*}
\begin{equation*}
<\hat{T}>=\left<\frac{\hat{p}^2}{2m}\right>
\end{equation*}
\begin{equation*}
<\hat{Q}>=\sum_{n}q_n|c_n|^2
\end{equation*}
\begin{equation*}
<j>=\frac{\sum jN(j)}{N}=\sum_{j=0}^{\infty}jP(j)
\end{equation*}
\begin{equation*}
<j^2>=\sum_{j=0}^{\infty}j^2P(j)
\end{equation*}
\begin{equation*}
<f(j)>=\sum_{j=0}^{\infty}f(j)P(j)
\end{equation*}
\begin{equation*}
\frac{d}{dt}<\hat{Q}>=\frac{i}{\hbar}<[\hat{H},\hat{Q}]>+\left<\frac{\partial \hat{Q}}{\partial t}\right>
\end{equation*}
\begin{equation*}
<H>=E
\end{equation*}
\begin{equation*}
<H^2>=E^2
\end{equation*}
\begin{equation*}
<H>=\sum_{n=1}^{\infty} |C_n|^2E_n
\end{equation*}
\begin{equation*}
\sigma=\sqrt{<j^2>-<j>^2}
\end{equation*}
\begin{equation*}
\sigma^2=<(\Delta x^2)>
\end{equation*}
\begin{equation*}
p=\frac{h}{\lambda}=\frac{2\pi \hbar}{\lambda}
\end{equation*}
\begin{equation*}
\sigma_x\sigma_p\geq\frac{\hbar}{2}
\end{equation*}
\begin{equation*}
\Delta t\Delta E \geq \frac{\hbar}{2}
\end{equation*}
\begin{equation*}
\sigma_{A}^{2}\sigma_{B}^{2} \geq \left(\frac{1}{2i}<[\hat{A},\hat{B}]>\right)^2
\end{equation*}
\begin{equation*}
\hat{E}=i\hbar\frac{\partial \Psi}{\partial t}
\end{equation*}
\begin{equation*}
\hat{p}=\frac{\hbar}{i}\frac{\partial}{\partial x}
\end{equation*}
\begin{equation*}
\hat{T}=\frac{\hat{p}^2}{2m}
\end{equation*}
\begin{equation*}
\hat{H}=\frac{-\hbar^2}{2m}\frac{\partial^2}{\partial x^2}+V(x)
\end{equation*}
\begin{equation*}
\phi(t)=e^{-iE_nt/\hbar}
\end{equation*}
\begin{equation*}
\Psi(x,t)=\Psi(x)\phi(t)
\end{equation*}
\begin{equation*}
\Psi(x,t)=\Psi(x)e^{-iE_nt/\hbar}
\end{equation*}
\begin{equation*}
\Psi_n(r,t)=\Psi_n(r)e^{-iE_nt/\hbar}
\end{equation*}
\begin{equation*}
\Psi(r,t)=\sum C_n\Psi_n(r)e^{-iE_nt\hbar}
\end{equation*}
\begin{equation*}
\Psi(x,t)=\sum_{n=1}^{\infty}c_n\Psi_n(x)e^{-iE_nt/\hbar}
\end{equation*}
\begin{equation*}
\phi(k)=\frac{1}{\sqrt{2\pi}}\int_{-\infty}^{\infty}\Psi(x,0)e^{-ikx} \ dx
\end{equation*}
\begin{equation*}
\Psi(x,t)=\frac{1}{\sqrt{2\pi}}\int_{-\infty}^{\infty}\phi(k)e^{i\left(kx-\frac{\hbar k^2}{2m}t\right)} \ dk
\end{equation*}
\begin{equation*}
\Psi(x,t)=\frac{\sqrt{m\alpha}}{\hbar}e^{-m\alpha|x|/\hbar^2}e^{-iEt/\hbar}
\end{equation*}
\begin{equation*}
\phi(p,t)=\frac{1}{2\pi\hbar}\int_{-\infty}^{\infty}e^{-ipx/\hbar}\Psi(x,t) \ dx
\end{equation*}
\begin{equation*}
\phi(x,t)=\frac{1}{2\pi\hbar}\int_{-\infty}^{\infty}e^{-ipx/\hbar}\Psi(p,t) \ dp
\end{equation*}
\begin{equation*}
E_n=\frac{\hbar^2k_{n}^{2}}{2m}=\frac{n^2\pi^2\hbar^2}{2ma^2} \ \text{\tiny (I.S.W)} 
\end{equation*}
\begin{equation*}
\Psi_n(x)=\sqrt{\frac{2}{a}}\sin{\left(\frac{n\pi}{a}x\right)} \ \text{\tiny (I.S.W)}
\end{equation*}
\begin{equation*}
\int \Psi_{m}^{*}(x)\Psi_{n}(x)  \ dx=\delta_{mn}
\end{equation*}
\begin{equation*}
C_n=\int \Psi_{n}^{*}(x)\Psi(x,0)  \ dx 
\end{equation*}
\begin{equation*}
C_n=<f_n|\Psi>=\int f_n(x)^{*}\Psi(x,0)  \ dx
\end{equation*}
\begin{equation*}
V(x)=\frac{1}{2}mw^2x^2 \ \text{\tiny (H.O)}
\end{equation*}
\begin{equation*}
[x,p]=i\hbar
\end{equation*}
\begin{equation*}
[\hat{x},\hat{p}]=i\hbar
\end{equation*}
\begin{equation*}
E_n=(n+1/2)\hbar w \ \text{\tiny (H.O)}
\end{equation*}
\begin{equation*}
a_{\pm}=\frac{1}{\sqrt{2\hbar mw}}(\mp ip+mwx)
\end{equation*}
\begin{equation*}
a_+\Psi_n=\sqrt{n+1}\Psi_{n+1}
\end{equation*}
\begin{equation*}
a_-\Psi_n=\sqrt{n}\Psi_{n-1}
\end{equation*}
\begin{equation*}
(a_+)^2\Psi_n \ \propto \ \Psi_{n+2}
\end{equation*}
\begin{equation*}
(a_-)^2\Psi_n \ \propto \ \Psi_{n-2}
\end{equation*}
\begin{equation*}
a_+a_-\Psi_n=n\Psi_n
\end{equation*}
\begin{equation*}
a_-a_+\Psi_n=(n+1)\Psi_n
\end{equation*}
\begin{equation*}
a_-\Psi_0=0
\end{equation*}
\begin{equation*}
\Psi_0(x)=\left(\frac{mw}{\pi \hbar}\right)^{\frac{1}{4}}e^{\frac{-mw}{2\hbar}x^2}
\end{equation*}
\begin{equation*}
\Psi_n(x)=A_n(a_+)^n\Psi_0(x)
\end{equation*}
\begin{equation*}
\Psi_n=\frac{(a_+)^n}{\sqrt{n!}}\Psi_0
\end{equation*}
\begin{equation*}
x=\sqrt{\frac{\hbar}{2mw}}(a_++a_-)
\end{equation*}
\begin{equation*}
\hat{p}=i\sqrt{\frac{\hbar mw}{2}}(a_+-a_-)
\end{equation*}
\begin{equation*}
R=(1+(2\hbar^2E/m\alpha^2))^{-1}
\end{equation*}
\begin{equation*}
T=(1+(m\alpha^2/2\hbar^2E))^{-1}
\end{equation*}
\begin{equation*}
R=\frac{|B|^2}{|A|^2} ,\ T=\frac{|F|^2}{|A|^2}
\end{equation*}
\begin{equation*}
R+T=1
\end{equation*}
\begin{equation*}
|\alpha> \rightarrow a=
\begin{pmatrix}
a_1 \\ a_2 \\ a_3
\end{pmatrix}
\end{equation*}
\begin{equation*}
<\alpha| \rightarrow a^{*}=
\begin{pmatrix}
a_{1}^{*} & a_{2}^{*} & a_{3}^{*}
\end{pmatrix}
\end{equation*}
\begin{equation*}
\text{\tiny H.S iff} <\beta|\alpha>=<\alpha|\beta>^{*}
\end{equation*}
\begin{equation*}
<\alpha|\alpha>=\int_{a}^{b}|f(x)|^2 \ dx
\end{equation*}
\begin{equation*}
<f_m|f_n>=\delta_{mn}
\end{equation*}
\begin{equation*}
<\hat{A}>=<\delta(0)|\hat{A}|\delta(0)>
\end{equation*}
\begin{equation*}
P=|<\lambda_n|\delta(t)>|^2
\end{equation*}
\begin{equation*}
|\delta(t)>=\phi(t)|\delta(0)>
\end{equation*}
\begin{equation*}
|\delta(0)>=|\lambda_n>
\end{equation*}
\begin{equation*}
\Psi(x,t)=<x|\delta(t)>
\end{equation*}
\begin{equation*}
\phi(p,t)=<p|\delta(t)>
\end{equation*}
\begin{equation*}
C_n(t)=<n|\delta(t)>
\end{equation*}
\begin{equation*}
\hat{Q}_{mn}=<e_m|\hat{Q}|e_n>
\end{equation*}
\begin{equation*}
i\hbar\frac{d}{dt}|\delta>=H|\delta>
\end{equation*}
\begin{equation*}
\hat{H}|\delta>=E|\delta>
\end{equation*}
\begin{equation*}
\hat{P}=|\alpha><\alpha|
\end{equation*}
\begin{equation*}
\hat{P}|\delta>=<\alpha|\beta|\alpha>
\end{equation*}
\begin{equation*}
<e_m|e_n>=\delta_{mn}
\end{equation*}
\begin{equation*}
p_x=\frac{\hbar}{i}\frac{\partial}{\partial x} ,\ p_y=\frac{\hbar}{i}\frac{\partial}{\partial x} ,\ p_z=\frac{\hbar}{i}\frac{\partial}{\partial z}
\end{equation*}
\begin{equation*}
p=\frac{\hbar}{i}\nabla
\end{equation*}
\begin{equation*}
P_{l}(x)=\frac{1}{2^ll!}\left(\frac{d}{dx}\right)^l(x^2-1)^l
\end{equation*}
\begin{equation*}
P_{l}^{m}(x)=(1-x^2)^{|m|/2}\left(\frac{d}{dx}\right)^{|m|}P_{l}(x)
\end{equation*}
\begin{equation*}
\begin{split}
Y_{l}^{m}(\theta,\phi)=&\Bigg[\epsilon\sqrt{\frac{(2l+1)}{(4\pi)}\frac{(l-|m|)!}{(l+|m|)!}} \\
&\times e^{im\phi} \ P_{l}^{m}(\cos{\theta})\Bigg],\hspace{5pt} \epsilon=(-1)^m 
\end{split}
\end{equation*}
\begin{equation*}
j_l(x)=(-x)^l\left(\frac{1}{x}\frac{d}{dx}\right)\frac{\sin{(x)}}{x}
\end{equation*}
\begin{equation*}
n_l(x)=-(-x)^l\left(\frac{1}{x}\frac{d}{dx}\right)^l\frac{\cos{(x)}}{x}
\end{equation*}
\begin{equation*}
E_n=-\left[\frac{m}{2\hbar^2}\left(\frac{e^2}{4\pi\epsilon_0}\right)^2\right]\frac{1}{n^2}=\frac{E_1}{n^2}
\end{equation*}
\begin{equation*}
\Psi_{100}(r,\theta,\phi)=\frac{e^{-r/a}}{\sqrt{\pi a^3}}
\end{equation*}
\begin{equation*}
\begin{split}
\Psi_{nlm}=&\Bigg[\sqrt{\left(\frac{2}{na}\right)^3\frac{(n-l-1)!}{2n[(n+1)!]^3}} \ e^{-r/na} \\
&\times\Big(\frac{2r}{na}\Big)^l\left[L_{n-l-1}^{2l+1}\Big(\frac{2r}{na}\Big)\right]Y_{l}^{m}(\theta,\phi)\Bigg]
\end{split}
\end{equation*}
\begin{equation*}
\Delta E=E_1\left(\frac{1}{n_{f}^{2}}-\frac{1}{n_{i}^{2}}\right)
\end{equation*}
\begin{equation*}
\frac{1}{\lambda}=R\left(\frac{1}{n_{f}^{2}}-\frac{1}{n_{i}^{2}}\right)
\end{equation*}
\begin{equation*}
P=\int_{0}^{2\pi}\int_{0}^{\pi}\int_{0}^{\infty}\left(f(r)\right)^2r^2\sin^2{(\theta)} \ dr d\theta d\phi
\end{equation*}
\begin{equation*}
\eta=\int_{0}^{2\pi}\int_{0}^{\pi}f(r,\theta,\phi)^*f(r,\theta,\phi) \ \sin{(\theta)}\  d\theta d\phi
\end{equation*}
\begin{equation*}
\mathcal{O}=\int_{0}^{2\pi}\int_{0}^{\pi}f(r,\theta,\phi)^*f(r,\theta,\phi) \sin{(\theta)}\ d\theta d\phi 
\end{equation*}
\begin{equation*}
L=r \ \textbf{x} \ p
\end{equation*}
\begin{equation*}
L_{x}=yP_z-zP_y
\end{equation*}
\begin{equation*}
L_{y}=zP_x-xP_z
\end{equation*}
\begin{equation*}
L_{z}=xP_y-yP_x
\end{equation*}
\begin{equation*}
[L_x,L_y]=i\hbar L_z
\end{equation*}
\begin{equation*}
[L_y,L_z]=i\hbar L_x
\end{equation*}
\begin{equation*}
[L_z,L_x]=i\hbar L_y
\end{equation*}
\begin{equation*}
[L^2,L]=0
\end{equation*}
\begin{equation*}
L_{\pm}=L_x\pm iL_y
\end{equation*}
\begin{equation*}
L^{2}f_{l}^{m}=\hbar^2l(l+1)f_{l}^{m}
\end{equation*}
\begin{equation*}
L_zf_{l}^{m}=\hbar m f_{l}^{m}
\end{equation*}
\begin{equation*}
L_z=\frac{\hbar}{i}\frac{\partial}{\partial \phi}
\end{equation*}
\begin{equation*}
L_{\pm}=\pm\hbar e^{\pm i \phi}\left(\frac{\partial}{\partial \theta} \pm i\cot{\theta}\frac{\partial}{\partial \phi}\right)
\end{equation*}
\begin{equation*}
L^2=-\hbar^2\left[\frac{1}{\sin{\theta}}\frac{\partial}{\partial \theta}\left(\sin{\theta}\frac{\partial}{\partial \theta}\right)+\frac{1}{\sin^2{\theta}}\frac{\partial^2}{\partial \phi^2}\right]
\end{equation*}
\begin{equation*}
[s_x,s_y]=i\hbar s_z
\end{equation*}
\begin{equation*}
[s_y,s_z]=i\hbar s_x
\end{equation*}
\begin{equation*}
[s_z,s_x]=i\hbar s_y
\end{equation*}
\begin{equation*}
S^2=\frac{3}{4}\hbar^2
\begin{pmatrix}
1 & 0 \\ 0 & 1
\end{pmatrix}
\end{equation*}
\begin{equation*}
S_x=\frac{\hbar}{2}
\begin{pmatrix}
0 & 1 \\ 1 & 0
\end{pmatrix}
\end{equation*}
\begin{equation*}
S_y=\frac{\hbar}{2}
\begin{pmatrix}
0 & -i \\ i & 0
\end{pmatrix}
\end{equation*}
\begin{equation*}
S_z=\frac{\hbar}{2}
\begin{pmatrix}
1 & 0 \\ 0 & -1
\end{pmatrix}
\end{equation*}
\begin{equation*}
\chi=
\begin{pmatrix}
a \\ b
\end{pmatrix}
=a\chi_++b\chi_-
\end{equation*}
\begin{equation*}
\chi_+=
\begin{pmatrix}
1 \\ 0
\end{pmatrix}
,\ \lambda=\frac{\hbar}{2}
\end{equation*}
\begin{equation*}
\chi_-=
\begin{pmatrix}
0 \\ 1
\end{pmatrix}
,\ \lambda=\frac{-\hbar}{2}
\end{equation*}
\begin{equation*}
\chi_{+}^{(x)}=\frac{1}{\sqrt{2}}=
\begin{pmatrix}
1 \\ 1
\end{pmatrix}
,\ \lambda=\frac{\hbar}{2}
\end{equation*}
\begin{equation*}
\chi_{-}^{(x)}=\frac{1}{\sqrt{2}}
\begin{pmatrix}
1 \\ -1
\end{pmatrix}
,\ \lambda=\frac{-\hbar}{2}
\end{equation*}
\begin{equation*}
\chi_{+}^{(y)}=\frac{1}{\sqrt{2}}=
\begin{pmatrix}
1 \\ i
\end{pmatrix}
,\ \lambda=\frac{\hbar}{2}
\end{equation*}
\begin{equation*}
\chi_{-}^{(y)}=\frac{1}{\sqrt{2}}=
\begin{pmatrix}
1 \\ -i
\end{pmatrix}
,\ \lambda=\frac{-\hbar}{2}
\end{equation*}
\begin{equation*}
\chi_{+}^{(z)}=\frac{1}{\sqrt{2}}=
\begin{pmatrix}
1 \\ 0
\end{pmatrix}
,\ \lambda=\frac{\hbar}{2}
\end{equation*}
\begin{equation*}
\chi_{-}^{(z)}=\frac{1}{\sqrt{2}}=
\begin{pmatrix}
0 \\ 1
\end{pmatrix}
,\ \lambda=\frac{-\hbar}{2}
\end{equation*}
\begin{equation*}
\chi=\left(\frac{a+b}{\sqrt{2}}\right)\chi_{+}^{(i)}+\left(\frac{a-b}{\sqrt{2}}\right)\chi_{-}^{(i)}
\end{equation*}
\begin{equation*}
\chi(t)=
\begin{pmatrix}
\cos{(\alpha/2)}e^{i\gamma B_{0}t/2} \\ \sin{(\alpha/2)}e^{-i\gamma B_{0}t/2}
\end{pmatrix}
\end{equation*}
\begin{equation*}
<S>=\chi^{*}S\chi
\end{equation*}
\begin{equation*}
\eta=\chi^{*}\chi=1
\end{equation*}
\begin{equation*}
\textbf{H}=-\mu \cdot \textbf{B}=-\gamma \textbf{B} \cdot \textbf{S}
\end{equation*}
\begin{equation*}
P_{\pm}^{(i)}=|C_{\pm}^{(i)}|^2
\end{equation*}
\begin{equation*}
C_{\pm}^{(i)}=\chi_{\pm}^{(i)^{*}}\chi_{\pm}
\end{equation*}
\begin{equation*}
i\hbar\frac{\partial \chi}{\partial t}=H\chi
\end{equation*}
\end{multicols}
%---------------------------------------------------------------------------
%	Mathematical Equations and Constants
%---------------------------------------------------------------------------
\begin{center}
\underline{\textbf{Mathematical Equations and Constants}}
\end{center}
\begin{equation*}
\int_{0}^{\infty}x^ne^{-x/a}dx=n!a^{n+1},
\hspace{10pt}
\int_{0}^{\infty}x^{2n}e^{-x^2/a^x}dx=\sqrt{\pi}\frac{(2n)!}{n!}\left(\frac{a}{2}\right)^{2n+1},
\hspace{10pt}
\int_{0}^{\infty}x^{2n+1}e^{-x^2/a^2}dx=\frac{n!}{2}a^{2n+2}
\end{equation*}
\begin{equation*}
\nabla^2=\frac{1}{r^2}\frac{\partial}{\partial r}\left(r^2\frac{\partial f}{\partial r}\right)+\frac{1}{r^2\sin{\theta}}\frac{\partial}{\partial \theta}\left(\sin{\theta}\frac{\partial f}{\partial \theta}\right)+\frac{1}{r^2\sin^2{\theta}}\frac{\partial^2 f}{\partial \phi^2}
\hspace{10pt}:\hspace{10pt}
a\ddot{x}+b\dot{x}+x=0, \hspace{10pt} \Delta=b^2-4ac
\end{equation*}
\begin{equation*}
\text{\tiny iff} \ \Delta>0, \hspace{5pt} x(t)=Ae^{r_1t}+Be^{r_2t}: \hspace{10pt}
\text{\tiny iff} \ \Delta=0, \hspace{5pt} x(t)=Ae^{rt}+Bte^{rt}: \hspace{10pt}
\text{\tiny iff} \ \Delta<0, \hspace{5pt} x(t)=Ae^{irt}+Be^{-irt}
\end{equation*}
\begin{equation*}
E_1=-13.6 \ \text{ev}, \hspace{5pt}
R=1.097\cdot10^7 \ \text{m$^{-1}$}, \hspace{5pt}
\hbar=1.05457\cdot10^{-34} \ \text{Js}, \hspace{5pt}
c=2.99792\cdot10^8 \ \text{m/s}, \hspace{5pt}
m_e=9.10938\cdot10^{-31} \ \text{Kg}
\end{equation*}
\begin{equation*}
m_p=1.67262\cdot10^{-27} \ \text{Kg}, \hspace{5pt}
e_{+,-}=\pm1.67262\cdot10^{-19} \ \text{C}, \hspace{5pt}
\epsilon_{0}=8.85419\cdot10^{-12} \ \text{C$^2$/Jm}, \hspace{5pt}
k_{B}=1.38065\cdot10^{-23} \ \text{J/K}
\end{equation*}
\begin{equation*}
[x^2+y,z]=[x^2,z]+[y,z],
\hspace{5pt}
[x^2,z]=x[x,z]+[x,z]x,
\hspace{5pt}
[A,B]=AB-BA,
\hspace{5pt}
[\hat{A},\hat{B}]=\hat{A}\hat{B}-\hat{B}\hat{A}
\hspace{5pt}
\end{equation*}
\newpage
%---------------------------------------------------------------------------
%	Helpful Hints
%---------------------------------------------------------------------------
\begin{center}
\underline{\textbf{Helpful Hints}}
\end{center}
\begin{multicols}{2}
\begin{equation*}
\begin{split}
\text{Discrete Values:} \\
C_n=&<\Psi_n|\Psi(x,0)|> \\
\Psi(x,t)=&\sum C_ne^{-iE_nt/\hbar} \\
<\Psi_m|\Psi_n>=& \ \delta_{mn}
\end{split}
\hspace{20pt}
\begin{split}
\text{Continuous Values:} \\
\phi(k)=&<F_{P}^{i}|\Psi(x,t)> \\
\Psi(x,t)=&<\phi(k)|F_Pe^{-iE_nt/\hbar}> \\
<F_p|F_p>=& \ \delta(P-P')
\end{split}
\end{equation*}
\end{multicols}
\begin{itemize}
\item{Schr\"odingers equation solves for a spinless, nonrelativistic, quantum mechanical system.}
\item{Discrete values are finite and can be known. i.e Energies.}
\item{Unbound energies have continuous spectrum of Eigenvalues.}
\item{Continus values are probabilities. i.e Position and Momentum.}
\item{Wave functions live in Hilbert Space.}
\item{Finite inner products indicate that the wave function given lives in Hilbert space.}
\item{Observables are represented by hermitian operators.}
\item{Operators in Quantum Mechanics represent physically observable quantities.}
\item{Determinate States: Every measurement of $\hat{Q}$ returns the same value q.}
\item{Determinate States are eigenfunctions of $\hat{Q}$.}
\end{itemize}
\end{document}